modal companion of minimum/maximal MC and rewrite int

Foundation/Modal/ModalCompanion/Basic.lean
@@ -22,9 +22,146 @@ class Modal.ModalCompanion (IL : Propositional.Logic) (ML : Modal.Logic) where
 lemma Modal.instModalCompanion (h₁ : ∀ {φ}, φ ∈ IL → φᵍ ∈ ML) (h₂ : ∀ {φ}, φᵍ ∈ ML → φ ∈ IL) : Modal.ModalCompanion IL ML := ⟨λ {_} => ⟨h₁, h₂⟩⟩
 
 
-def Propositional.Logic.minimamMC (IL : Propositional.Logic) : Modal.Logic := Modal.Logic.sumNormal Modal.Logic.S4 { φᵍ | φ ∈ IL }
+namespace Propositional.Logic
 
-def Propositional.Logic.maximalMC (IL : Propositional.Logic) : Modal.Logic := Modal.Logic.addNormal IL.minimamMC (Axioms.Grz (.atom 0))
+def minimamMC (IL : Propositional.Logic) : Modal.Logic := Modal.Logic.sumNormal Modal.Logic.S4 { φᵍ | φ ∈ IL }
+
+def maximalMC (IL : Propositional.Logic) : Modal.Logic := Modal.Logic.addNormal IL.minimamMC (Axioms.Grz (.atom 0))
+
+/-
+lemma minimanMC_Hilbert (H : Hilbert ℕ) : H.logic.minimamMC = Modal.Logic.sumNormal Modal.Logic.S4 { φᵍ | φ ∈ H.axiomInstances } := by
+  ext φ;
+  constructor;
+  . rintro h;
+    unfold Hilbert.logic minimamMC at h;
+    induction h with
+    | mem₁ h => exact Modal.Logic.sumNormal.mem₁ h;
+    | mdp hφ hψ ihφ ihψ => apply Modal.Logic.sumNormal.mdp ihφ ihψ;
+    | subst h ih => apply Modal.Logic.sumNormal.subst ih;
+    | nec h ih => apply Modal.Logic.sumNormal.nec ih;
+    | mem₂ h =>
+      apply Modal.Logic.sumNormal.mem₂;
+      obtain ⟨φ, hφ, rfl⟩ := h;
+      use φ;
+      simp at hφ;
+  . sorry;
+-/
+
+end Propositional.Logic
+
+
+section
+
+open Propositional.Formula (goedelTranslate)
+
+lemma Modal.instModalCompanion_of_minimamMC_via_KripkeSemantics
+  {IL : Propositional.Logic}
+  (IC : Propositional.Kripke.FrameClass) (hIL_complete : ∀ {φ}, φ ∈ IL ↔ φ ∈ IC.logic)
+  (MC : Modal.Kripke.FrameClass) (hML_complete : ∀ {φ}, φ ∈ IL.minimamMC ↔ φ ∈ MC.logic)
+  (hIC_MC : ∀ F ∈ IC, ⟨F.World, F.Rel⟩ ∈ MC)
+  : ModalCompanion IL (IL.minimamMC) := Modal.instModalCompanion
+  (by
+    intro φ hφ;
+    apply Modal.Logic.sumNormal.mem₂;
+    use φ;
+  )
+  (by
+    intro φ;
+    contrapose;
+    intro h;
+    have := hIL_complete.not.mp h;
+    obtain ⟨F, hF, hF₂⟩ := by simpa using this;
+    obtain ⟨V, x, hφ⟩ := Propositional.Formula.Kripke.ValidOnFrame.exists_valuation_world_of_not hF₂;
+    have h₁ : ∀ ψ x, Propositional.Formula.Kripke.Satisfies ⟨F, V⟩ x ψ ↔ (Modal.Formula.Kripke.Satisfies ⟨⟨F.World, F.Rel⟩, V⟩ x (ψᵍ)) := by
+      intro ψ x;
+      induction ψ using Propositional.Formula.rec' generalizing x with
+      | hatom a =>
+        unfold goedelTranslate;
+        constructor;
+        . intro _ _ h;
+          exact V.hereditary h $ by assumption;
+        . intro h;
+          exact h x (F.rel_refl x);
+      | hfalsum =>  rfl;
+      | hor φ ψ ihp ihq =>
+        unfold goedelTranslate;
+        constructor;
+        . rintro (hp | hq);
+          . apply Modal.Formula.Kripke.Satisfies.or_def.mpr; left;
+            exact ihp x |>.mp hp;
+          . apply Modal.Formula.Kripke.Satisfies.or_def.mpr; right;
+            exact ihq x |>.mp hq;
+        . intro h;
+          rcases Modal.Formula.Kripke.Satisfies.or_def.mp h with (hp | hq)
+          . left; exact ihp x |>.mpr hp;
+          . right; exact ihq x |>.mpr hq;
+      | _ => simp_all [goedelTranslate, Propositional.Formula.Kripke.Satisfies, Modal.Formula.Kripke.Satisfies];
+    apply hML_complete.not.mpr;
+    apply Modal.Formula.Kripke.ValidOnFrameClass.not_of_exists_frame;
+    use { World := F.World, Rel := F.Rel };
+    constructor;
+    . apply hIC_MC;
+      exact hF;
+    . apply Modal.Formula.Kripke.ValidOnFrame.not_of_exists_valuation_world;
+      use V, x;
+      exact (h₁ φ x).not.mp hφ;
+  )
+
+lemma Modal.instModalCompanion_of_maximalMC_via_KripkeSemantics
+  {IL : Propositional.Logic}
+  (IC : Propositional.Kripke.FrameClass) (hIL_complete : ∀ {φ}, φ ∈ IL ↔ φ ∈ IC.logic)
+  (MC : Modal.Kripke.FrameClass) (hML_complete : ∀ {φ}, φ ∈ IL.maximalMC ↔ φ ∈ MC.logic)
+  (hIC_MC : ∀ F ∈ IC, ⟨F.World, F.Rel⟩ ∈ MC)
+  : ModalCompanion IL (IL.maximalMC) := Modal.instModalCompanion
+  (by
+    intro φ hφ;
+    apply Modal.Logic.sumNormal.mem₁;
+    apply Modal.Logic.sumNormal.mem₂;
+    use φ;
+  )
+  (by
+    intro φ;
+    contrapose;
+    intro h;
+    have := hIL_complete.not.mp h;
+    obtain ⟨F, hF, hF₂⟩ := by simpa using this;
+    obtain ⟨V, x, hφ⟩ := Propositional.Formula.Kripke.ValidOnFrame.exists_valuation_world_of_not hF₂;
+    have h₁ : ∀ ψ x, Propositional.Formula.Kripke.Satisfies ⟨F, V⟩ x ψ ↔ (Modal.Formula.Kripke.Satisfies ⟨⟨F.World, F.Rel⟩, V⟩ x (ψᵍ)) := by
+      intro ψ x;
+      induction ψ using Propositional.Formula.rec' generalizing x with
+      | hatom a =>
+        unfold goedelTranslate;
+        constructor;
+        . intro _ _ h;
+          exact V.hereditary h $ by assumption;
+        . intro h;
+          exact h x (F.rel_refl x);
+      | hfalsum =>  rfl;
+      | hor φ ψ ihp ihq =>
+        unfold goedelTranslate;
+        constructor;
+        . rintro (hp | hq);
+          . apply Modal.Formula.Kripke.Satisfies.or_def.mpr; left;
+            exact ihp x |>.mp hp;
+          . apply Modal.Formula.Kripke.Satisfies.or_def.mpr; right;
+            exact ihq x |>.mp hq;
+        . intro h;
+          rcases Modal.Formula.Kripke.Satisfies.or_def.mp h with (hp | hq)
+          . left; exact ihp x |>.mpr hp;
+          . right; exact ihq x |>.mpr hq;
+      | _ => simp_all [goedelTranslate, Propositional.Formula.Kripke.Satisfies, Modal.Formula.Kripke.Satisfies];
+    apply hML_complete.not.mpr;
+    apply Modal.Formula.Kripke.ValidOnFrameClass.not_of_exists_frame;
+    use { World := F.World, Rel := F.Rel };
+    constructor;
+    . apply hIC_MC;
+      exact hF;
+    . apply Modal.Formula.Kripke.ValidOnFrame.not_of_exists_valuation_world;
+      use V, x;
+      exact (h₁ φ x).not.mp hφ;
+  )
+
+end
 
 /-
 lemma dp_of_mdp [ModalDisjunctive mH] [ModalCompanion iH mH] [Entailment.S4 mH] : iH ⊢! φ ⋎ ψ → iH ⊢! φ ∨ iH ⊢! ψ := by
