Foundation/Modal/ModalCompanion/Int.lean
@@ -1,6 +1,7 @@
 import Foundation.Modal.ModalCompanion.Basic
 import Foundation.Propositional.Logic.WellKnown
 import Foundation.Modal.Logic.WellKnown
+import Foundation.Modal.Logic.Extension
 import Foundation.Modal.Logic.Sublogic.Grz
 
 namespace LO.Modal
@@ -74,46 +75,49 @@ lemma Logic.gS4_of_Int : φ ∈ Logic.Int → φᵍ ∈ Logic.S4 := by
   rintro _ ⟨φ, ⟨_⟩, ⟨s, rfl⟩⟩;
   apply nec! $ efq!;
 
-lemma Logic.Int_of_gS4 : φᵍ ∈ Logic.S4 → φ ∈ Logic.Int := by
-  contrapose;
-  rw [Logic.Int.eq_AllKripkeFrameClass_Logic, Logic.S4.eq_ReflexiveTransitiveKripkeFrameClass_Logic];
-  intro h;
-  obtain ⟨M, w, hM, hp⟩ := Propositional.Formula.Kripke.ValidOnFrameClass.exists_model_world_of_not h;
-  have h₁ : ∀ ψ x, Propositional.Formula.Kripke.Satisfies M x ψ ↔ (Modal.Formula.Kripke.Satisfies ⟨⟨M.World, M.Rel⟩, M.Val⟩ x (ψᵍ)) := by
-    intro ψ x;
-    induction ψ using Propositional.Formula.rec' generalizing x with
-    | hatom a =>
-      unfold goedelTranslate;
-      constructor;
-      . intro _ _ h;
-        exact M.Val.hereditary h $ by assumption;
-      . intro h;
-        exact h x (M.rel_refl x);
-    | hfalsum =>  rfl;
-    | hor φ ψ ihp ihq =>
-      unfold goedelTranslate;
-      constructor;
-      . rintro (hp | hq);
-        . apply Formula.Kripke.Satisfies.or_def.mpr; left;
-          exact ihp x |>.mp hp;
-        . apply Formula.Kripke.Satisfies.or_def.mpr; right;
-          exact ihq x |>.mp hq;
-      . intro h;
-        rcases Formula.Kripke.Satisfies.or_def.mp h with (hp | hq)
-        . left; exact ihp x |>.mpr hp;
-        . right; exact ihq x |>.mpr hq;
-    | _ => simp_all [goedelTranslate, Propositional.Formula.Kripke.Satisfies, Modal.Formula.Kripke.Satisfies];
-  apply Formula.Kripke.ValidOnFrameClass.not_of_exists_model;
-  use {World := M.World, Rel := M.Rel, Val := M.Val};
+lemma Logic.S4.is_minimamMC_of_Int : Logic.S4 = Logic.Int.minimamMC := by
+  ext φ;
   constructor;
-  . constructor;
-    . exact M.rel_refl;
-    . exact M.rel_trans;
-  . apply Formula.Kripke.ValidOnModel.not_of_exists_world;
-    use w;
-    exact (h₁ φ w).not.mp hp;
+  . intro hφ;
+    induction hφ using Hilbert.Deduction.rec! with
+    | maxm h =>
+      rcases (by simpa using h) with (⟨s, rfl⟩ | ⟨s, rfl⟩ | ⟨s, rfl⟩);
+      . apply Logic.sumNormal.mem₁; simp;
+      . apply Logic.sumNormal.mem₁; simp;
+      . apply Logic.sumNormal.mem₁; simp;
+    | mdp => apply Logic.sumNormal.mdp <;> assumption;
+    | nec => apply Logic.sumNormal.nec; assumption;
+    | _ => apply Logic.sumNormal.mem₁; simp;
+  . intro hφ;
+    induction hφ with
+    | mem₁ h => tauto;
+    | mdp hφ hψ ihφψ ihψ => apply Modal.Logic.mdp ihφψ ihψ;
+    | subst h ih => apply Modal.Logic.subst ih;
+    | nec h ih => apply Modal.Logic.nec ih;
+    | mem₂ h =>
+      rcases h with ⟨φ, hφ, rfl⟩;
+      apply Logic.gS4_of_Int hφ;
 
-instance : ModalCompanion Logic.Int Logic.S4 := Modal.instModalCompanion Logic.gS4_of_Int Logic.Int_of_gS4
+instance : ModalCompanion Logic.Int Logic.S4 := by
+  rw [Logic.S4.is_minimamMC_of_Int];
+  exact Modal.instModalCompanion_of_minimamMC_via_KripkeSemantics
+    (IC := Propositional.Kripke.AllFrameClass)
+    (MC := Modal.Kripke.ReflexiveTransitiveFrameClass)
+    (by
+      intro φ;
+      constructor;
+      . apply Propositional.Hilbert.Int.Kripke.sound.sound;
+      . apply Propositional.Hilbert.Int.Kripke.complete.complete;
+    )
+    (by
+      rw [←Logic.S4.is_minimamMC_of_Int];
+      intro φ;
+      constructor;
+      . apply Modal.Hilbert.S4.Kripke.sound.sound;
+      . apply Modal.Hilbert.S4.Kripke.complete.complete;
+    )
+    (fun F hF => ⟨F.rel_refl, F.rel_trans⟩);
+
 
 end S4
 
@@ -125,50 +129,57 @@ lemma Logic.gGrz_of_Int : φ ∈ Logic.Int → φᵍ ∈ Logic.Grz := by
   intro h;
   exact S4_ssubset_Grz.1 $ Logic.gS4_of_Int h;
 
-lemma Logic.Int_of_gGrz : φᵍ ∈ Logic.Grz → φ ∈ Logic.Int := by
-  contrapose;
-  rw [Logic.Int.eq_AllFiniteKripkeFrameClass_Logic, Logic.Grz.eq_ReflexiveTransitiveAntiSymmetricFiniteKripkeFrameClass_Logic];
-  intro h;
-  obtain ⟨M, w, hM, hp⟩ := Propositional.Formula.Kripke.ValidOnFrameClass.exists_model_world_of_not h;
-  have h₁ : ∀ ψ x, Propositional.Formula.Kripke.Satisfies M x ψ ↔ (Modal.Formula.Kripke.Satisfies ⟨⟨M.World, M.Rel⟩, M.Val⟩ x (ψᵍ)) := by
-    intro ψ x;
-    induction ψ using Propositional.Formula.rec' generalizing x with
-    | hatom a =>
-      unfold goedelTranslate;
-      constructor;
-      . intro _ _ h;
-        exact M.Val.hereditary h $ by assumption;
-      . intro h;
-        exact h x (M.rel_refl x);
-    | hfalsum =>  rfl;
-    | hor φ ψ ihp ihq =>
-      unfold goedelTranslate;
-      constructor;
-      . rintro (hp | hq);
-        . apply Formula.Kripke.Satisfies.or_def.mpr; left;
-          exact ihp x |>.mp hp;
-        . apply Formula.Kripke.Satisfies.or_def.mpr; right;
-          exact ihq x |>.mp hq;
-      . intro h;
-        rcases Formula.Kripke.Satisfies.or_def.mp h with (hp | hq)
-        . left; exact ihp x |>.mpr hp;
-        . right; exact ihq x |>.mpr hq;
-    | _ => simp_all [goedelTranslate, Propositional.Formula.Kripke.Satisfies, Modal.Formula.Kripke.Satisfies];
-  apply Formula.Kripke.ValidOnFrameClass.not_of_exists_model;
-  use {World := M.World, Rel := M.Rel, Val := M.Val};
+lemma Logic.Grz.is_maximalMC_of_Int : Logic.Grz = Logic.Int.maximalMC := by
+  ext φ;
   constructor;
-  . simp [ReflexiveTransitiveAntiSymmetricFiniteFrameClass, FiniteFrameClass.toFrameClass];
-    use ({ World := M.World, Rel := M.Rel, world_finite := by tauto; });
-    simp;
-    refine ⟨?_, ?_, ?_⟩;
-    . exact M.rel_refl;
-    . exact M.rel_trans;
-    . exact M.rel_antisymm;
-  . apply Formula.Kripke.ValidOnModel.not_of_exists_world;
-    use w;
-    exact (h₁ φ w).not.mp hp;
+  . intro hφ;
+    induction hφ using Hilbert.Deduction.rec! with
+    | maxm h =>
+      rcases (by simpa using h) with (⟨s, rfl⟩ | ⟨s, rfl⟩);
+      . apply Logic.sumNormal.mem₁;
+        apply Logic.sumNormal.mem₁;
+        simp;
+      . apply Logic.sumNormal.subst (φ := □(□((.atom 0) ➝ □(.atom 0)) ➝ (.atom 0)) ➝ (.atom 0)) (s := s);
+        apply Logic.sumNormal.mem₂;
+        simp;
+    | mdp => apply Logic.sumNormal.mdp <;> assumption;
+    | nec => apply Logic.sumNormal.nec; assumption;
+    | _ => apply Logic.sumNormal.mem₁; apply Logic.sumNormal.mem₁; simp;
+  . intro hφ;
+    induction hφ with
+    | mem₁ h =>
+      apply S4_ssubset_Grz.1;
+      rwa [Logic.S4.is_minimamMC_of_Int]
+    | mdp hφ hψ ihφψ ihψ => apply Modal.Logic.mdp ihφψ ihψ;
+    | subst h ih => apply Modal.Logic.subst ih;
+    | nec h ih => apply Modal.Logic.nec ih;
+    | mem₂ h =>
+      rcases h with ⟨φ, hφ, rfl⟩; simp;
 
-instance : ModalCompanion Logic.Int Logic.Grz := Modal.instModalCompanion Logic.gGrz_of_Int Logic.Int_of_gGrz
+instance : ModalCompanion Logic.Int Logic.Grz := by
+  rw [Logic.Grz.is_maximalMC_of_Int];
+  exact Modal.instModalCompanion_of_maximalMC_via_KripkeSemantics
+    (IC := Propositional.Kripke.AllFiniteFrameClass)
+    (MC := Modal.Kripke.ReflexiveTransitiveAntiSymmetricFiniteFrameClass)
+    (by
+      intro φ;
+      constructor;
+      . apply Propositional.Hilbert.Int.Kripke.sound_finite.sound;
+      . apply Propositional.Hilbert.Int.Kripke.complete_finite.complete;
+    )
+    (by
+      rw [←Logic.Grz.is_maximalMC_of_Int];
+      intro φ;
+      constructor;
+      . apply Modal.Hilbert.Grz.Kripke.sound.sound;
+      . apply Modal.Hilbert.Grz.Kripke.complete.complete;
+    )
+    (by
+      rintro F hF;
+      use ({ World := F.World, Rel := F.Rel, world_finite := by tauto; });
+      simp only [Set.mem_setOf_eq, and_true];
+      refine ⟨F.rel_refl, F.rel_trans, F.rel_antisymm⟩;
+    )
 
 end Grz
 
